:wrench: Add CWE cases

dataset/cwe-samples/task_id_1.dfy
@@ -1,14 +1,25 @@
 include "/Users/pari/pcc-llms/dataset/filesystems/interface/effectful-interface.dfy"
-method SafeJoin(path: seq<char>,  fname: seq<char>) returns (jointPath: path)
+
+function GetFileName(): string
 {
-  var fname := "public-key.txt";
+    // This method should return the filename
+    "public-key.txt"
+}
+
+function GetPath(): string
+{
+    // This method should return the path
+    "/documents"
+}
+
+method SafeJoin(path: seq<char>,  fname: seq<char>) returns (jointPath: path)
+requires path == GetPath()
+requires fname == GetFileName()
+{
   var f: FileStream;
   var ok: bool;
   ok, f := FileStream.Open(fname);
   if !ok { print "open failed\n"; return "";}
-  var path := "/documents";
   var joinIsOk:bool;
-  assert fname == "public-key.txt";
   joinIsOk, jointPath := f.Join(path, fname);
-  assert jointPath == "/documents/public-key.txt";
 }
