dataset/cwe-samples/task_id_3.dfy
@@ -1,17 +1,23 @@
 include "/Users/pari/pcc-llms/dataset/filesystems/interface/effectful-interface.dfy"
-method SafeRead(fname: seq<char>)
-// Prevents user from reading sensitive files or files without permission
-// Read with checking user permissions for reading the file
 
+function GetFileName(): string
 {
-    var fname := "safeFile-1.txt";
+    // This method should return the filename
+    "public-key.txt"
+}
+
+method SafeRead(fname: seq<char>)
+requires fname == GetFileName()
+{
     var f: FileStream;
     var ok: bool;
     ok, f := FileStream.Open(fname);
-    var user := "admin";
     if !ok { print "open failed\n"; return; }
     var data: array<byte> := new byte[100];
     ok := f.Read(fname, 0, data, 0, data.Length as int32);
     print "Safe Read operation!\n";
 
 }
+
+// Prevents user from reading sensitive files or files without permission
+// Read with checking user permissions for reading the file
